some more progress on relating pstep and tstep

examples/wysteria/sec_server.fst
@@ -1,6 +1,6 @@
 (*--build-config
-    options:--admit_fsi FStar.OrdSet --admit_fsi FStar.OrdMap --admit_fsi FStar.Set --admit_fsi Ffibridge --admit_fsi Runtime --admit_fsi FStar.IO --admit_fsi FStar.String --__temp_no_proj;
-    other-files:ghost.fst listTot.fst ordset.fsi ordmap.fsi classical.fst set.fsi heap.fst st.fst all.fst list.fst io.fsti string.fsi prins.fst ast.fst ffibridge.fsi sem.fst runtime.fsi print.fst ckt.fst interpreter.fst
+    options:--admit_fsi FStar.OrdSet --admit_fsi FStar.OrdMap --admit_fsi FStar.Set --admit_fsi Ffibridge --admit_fsi Runtime --admit_fsi FStar.IO --admit_fsi FStar.String --__temp_no_proj --admit_fsi FStar.Squash;
+    other-files:ghost.fst squash.fsti listTot.fst ordset.fsi ordmap.fsi classical.fst set.fsi heap.fst st.fst all.fst list.fst io.fsti string.fsi prins.fst ast.fst ffibridge.fsi sem.fst runtime.fsi print.fst ckt.fst interpreter.fst
  --*)
 
 module SecServer
@@ -23,6 +23,14 @@ type en_map = ordmap prin env p_cmp
 type out_map = ordmap prin chan_out p_cmp
 type redex_map = ordmap prin redex p_cmp
 
+
+(*
+ * ps   -- parties requires for this secure computation
+ * ps'  -- parties already checked-in
+ * pi   -- the protocol (mapping p to c) accumulated so far
+ * x,e  -- \x.e is the secure computation
+ * en_m -- the map of p |-> env accumulated so far
+ *)
 type tpre_assec' (ps:prins) (ps':prins) (pi:tpar ps') (x:varname) (e:exp) (en_m:en_map) =
   forall p. contains p pi ==>
        (contains p en_m /\
@@ -36,15 +44,19 @@ type tpre_assec' (ps:prins) (ps':prins) (pi:tpar ps') (x:varname) (e:exp) (en_m:
 	    MkTuple3._3 (get_en_b (R_assec.v r)) = e /\
 	    Some.v (select p en_m) = MkTuple3._1 (get_en_b (R_assec.v r)))))))
 
+(*
+ * Data type to accumulate the info for a secure computation as parties keep checking in
+ *)
 type psmap_v =
   | Mk_psmap:
     ps:prins -> ps':prins{subset ps' ps}
     -> en_m:en_map{forall p. mem p ps' = contains p en_m}
     -> out_m:out_map{forall p. mem p ps' = contains p out_m}
     -> red_m:redex_map{forall p. mem p ps' = contains p red_m}
-    -> x:varname -> e:exp
-    -> pi:tpar ps'{tpre_assec' ps ps' pi x e en_m /\
-                  (forall p. contains p pi ==> T_red.r (Conf.t (Some.v (select p pi))) = Some.v (select p red_m))}
+    -> x:varname
+    -> e:exp{exists (pi:tpar ps').
+              tpre_assec' ps ps' pi x e en_m /\
+              (forall p. contains p pi ==> T_red.r (Conf.t (Some.v (select p pi))) = Some.v (select p red_m))}
     -> psmap_v
 
 type psmap = ordmap prins psmap_v ps_cmp
@@ -55,20 +67,17 @@ type psmap_ref_t =
 
 (* private *) let psmap_ref = Mk_ref (alloc (OrdMap.empty #prins #psmap_v #ps_cmp))
 
-val do_sec_comp': c:config -> ML (c':config{is_sterminal c'} & (sstep_star c c'))
+(* call interpreter step_star on the input config *)
+val do_sec_comp':
+  c:config -> ML (c':config{is_sterminal c'} & (sstep_star c c'))
 let do_sec_comp' c =
   let (| c_opt, h |) = step_star c in
   if is_sterminal c_opt then
     (| c_opt, h |)
-    (* let T_val #meta v = Conf.t c_opt in *)
-    (* D_v meta v *)
   else
     failwith "Secure computation did not end in terminal state"
 
-assume val give_proof: #p:Type -> u:unit{p} -> Tot p
-assume val open_exists: #a:Type -> #p:(a -> Type) -> proof:(exists (x:a). p x) -> Tot (x:a & p x)
-assume val take_proof: #p:Type -> proof:p -> Tot (u:unit{p})
-
+(* convert a pi ->* pi' -> pi'' to pi ->* pi'' *)
 val pss_ps_to_pss:
   #ps:prins -> #pi:protocol ps -> #pi':protocol ps -> #pi'':protocol ps
   -> h1:pstep_star #ps pi pi' -> h2:pstep #ps pi' pi''
@@ -79,6 +88,7 @@ let rec pss_ps_to_pss #ps #pi #pi' #pi'' h1 h2 = match h1 with
     let hh = pss_ps_to_pss h2' h2 in
     PS_tran h1' hh
 
+(* that two protocols pi and pi' differ only in parties' terms *)
 type eq_proto' (ps:prins) (pi:tpar ps) (pi':tpar ps) =
   forall p. contains p pi ==>
        (Let (Some.v (select p pi))
@@ -90,6 +100,7 @@ type eq_proto' (ps:prins) (pi:tpar ps) (pi':tpar ps) =
            Conf.s c = Conf.s c' /\
            Conf.en c = Conf.en c'))))
 
+(* that pi contains slice of c's value for each party *)
 type final_prop (ps:prins) (pi:tpar ps) (c:config{is_value c}) =
   forall p. contains p pi ==>
        (Let (Conf.t (Some.v (select p pi)))
@@ -100,17 +111,7 @@ type final_prop (ps:prins) (pi:tpar ps) (c:config{is_value c}) =
 	   b2t (dvt = slice_v #(T_val.meta (Conf.t c)) p
 			      (T_val.v (Conf.t c)))))))
 
-type sec_prop =
-  | Mk_prop:
-    ps:prins -> x:varname -> e:exp
-    -> pi:tpar ps
-    -> c_sec_terminal:config{is_sterminal c_sec_terminal}
-    -> pi_init:protocol ps{pi_init = (pi, (OrdMap.empty #prins #tconfig_sec #ps_cmp)) /\ tpre_assec #ps pi_init ps x e}
-    -> pi_final:protocol ps
-    -> h:pstep_star #ps pi_init pi_final{final_prop ps (fst pi_final) c_sec_terminal /\
-                                        eq_proto' ps (fst pi_init) (fst pi_final)}
-    -> sec_prop
-
+(* that ret_sec_value_to_ps gives a final_prop protocol *)
 val ret_sec_value_to_ps_helper_lemma:
   #ps:prins
   -> pi:tpar ps{forall p. mem p ps ==>
@@ -121,72 +122,111 @@ val ret_sec_value_to_ps_helper_lemma:
           (ensures (final_prop ps pi' c))
 let ret_sec_value_to_ps_helper_lemma #ps pi c pi' = ()
 
+type pi_init_prop
+  (ps:prins) (pi:tpar ps) (en_m:en_map{forall p. mem p ps = contains p en_m})
+                          (red_m:redex_map{forall p. mem p ps = contains p red_m}) =
+  forall p. contains p pi ==>
+       (contains p en_m /\ contains p red_m /\
+        is_T_red (Conf.t (Some.v (select p pi))) /\
+	(Let (T_red.r (Conf.t (Some.v (select p pi))))
+	 (fun r -> is_R_assec r /\ is_clos (R_assec.v r) /\
+	        r = Some.v (select p red_m) /\
+	        MkTuple3._1 (get_en_b (R_assec.v r)) = Some.v (select p en_m))))
+  
+type sec_comp_prop
+  (ps:prins) (en_m:en_map{forall p. mem p ps = contains p en_m})
+  (red_m:redex_map{forall p. mem p ps = contains p red_m})
+  (x:varname) (e:exp) (c:config{is_sterminal c})
+  (pi_t: protocol ps * protocol ps) =
+
+  Let (fst pi_t)
+  (fun pi_init ->
+   (Let (snd pi_t)
+    (fun pi_final ->
+     pi_init_prop ps (fst pi_init) en_m red_m /\
+     tpre_assec #ps pi_init ps x e            /\
+     final_prop ps (fst pi_final) c           /\
+     pstep_star #ps pi_init pi_final          /\
+     eq_proto' ps (fst pi_init) (fst pi_final))))
+
+val init_sec_conf:
+  ps:prins -> en_m:en_map{contains_ps ps en_m} -> varname -> exp -> Tot tconfig_sec
+let init_sec_conf ps en_m x e =
+  Conf Target (Mode Sec ps) [] (update_env (compose_envs_m ps en_m) x V_unit)
+	      (T_exp e) (hide [])
+
+open FStar.Squash
+
 #set-options "--z3timeout 25"
 
 val create_pstep_star:
-  data:psmap_v{Equal (Mk_psmap.ps data) (Mk_psmap.ps' data)}
-  -> c_sec_terminal:config{is_sterminal c_sec_terminal}
-  -> h:sstep_star (Conf Target (Mode Sec (Mk_psmap.ps data)) []
-                       (update_env (compose_envs_m (Mk_psmap.ps data) (Mk_psmap.en_m data))
-		                   (Mk_psmap.x data) V_unit)
-		       (T_exp (Mk_psmap.e data)) (hide []))
-		 c_sec_terminal
-  -> Tot (p:sec_prop & (u:unit{Mk_prop.ps p = Mk_psmap.ps data /\
-                              Mk_prop.x p = Mk_psmap.x data   /\
-			      Mk_prop.e p = Mk_psmap.e data   /\
-			      Mk_prop.pi p = Mk_psmap.pi data}))
-let create_pstep_star data c_sec_terminal sstep_h =
-  let Mk_psmap ps _ en_m _ _ x e pi = data in
-
+  ps:prins -> en_m:en_map{forall p. mem p ps = contains p en_m}
+  -> red_m:redex_map{forall p.mem p ps = contains p red_m}
+  -> x:varname -> e:exp
+  -> c_sec:config{is_sterminal c_sec}
+  -> h:sstep_star (init_sec_conf ps en_m x e) c_sec
+  -> pi:tpar ps{tpre_assec' ps ps pi x e en_m /\
+               (forall p. contains p pi ==> T_red.r (Conf.t (Some.v (select p pi))) = Some.v (select p red_m))}
+  -> Tot (pi_t:(protocol ps * protocol ps) &
+         squash (sec_comp_prop ps en_m red_m x e c_sec pi_t))
+let create_pstep_star ps en_m red_m x e c_sec h pi =
   let pi_init = (pi, (OrdMap.empty #prins #tconfig_sec #ps_cmp)) in
-
-  let _ = cut (OrdMap.Equal (get_env_m #ps pi_init ps) en_m) in
+  let en_m' = get_env_m #ps pi_init ps in
+  let _ = cut (OrdMap.Equal en_m' en_m) in
 
   let pi_enter = tstep_assec #ps pi_init ps x e in
   let (pi_enter_par, pi_enter_sec) = pi_enter in
- 
-  let s1:pstep #ps pi_init pi_enter =
-    P_sec_enter #ps pi_init ps x e pi_enter in
 
-  let c_sec_init = Conf Target (Mode Sec ps) [] (update_env (compose_envs_m ps en_m) x V_unit) (T_exp e) (hide []) in
+  (* first step, enter secure block to pi_enter *)
+  let s1:pstep #ps pi_init pi_enter = P_sec_enter #ps pi_init ps x e pi_enter in
+  
+  let c_sec_init = init_sec_conf ps en_m x e in
 
-  let _ = cut (b2t (pi_enter_sec = update ps c_sec_init (snd pi_init))) in
+  //let _ = cut (b2t (pi_enter_sec = update ps c_sec_init (snd pi_init))) in
 
-  let _ = sec_comp_step_star_same_mode #c_sec_init #c_sec_terminal sstep_h in
+  sec_comp_step_star_same_mode #c_sec_init #c_sec h;
 
   //let _ = cut (is_sec c_sec_terminal /\ Conf.l c_sec_terminal = Target) in
 
-  let tsec_terminal:tsec = update ps c_sec_terminal (snd pi_init) in
+  let tsec_terminal:tsec = update ps c_sec (snd pi_init) in
   let pi_sec_terminal:(protocol ps) = (pi_enter_par, tsec_terminal) in
-  
-  let ss:pstep_star #ps pi_enter pi_sec_terminal =
-    sec_sstep_star_to_pstep_star c_sec_init c_sec_terminal sstep_h ps pi_enter_par (snd pi_init) in
 
-  let _ = cut (b2t (contains ps (snd pi_sec_terminal))) in
-  let _ = cut (b2t (Some.v (select ps (snd pi_sec_terminal)) = c_sec_terminal)) in
+  (* steps taken in secure computation *)
+  let ss:pstep_star #ps pi_enter pi_sec_terminal =
+    sec_sstep_star_to_pstep_star c_sec_init c_sec h ps pi_enter_par (snd pi_init) in
+
+  let _ = cut (b2t (Some.v (select ps (snd pi_sec_terminal)) = c_sec)) in
+
   //let _ = cut (b2t (Conf.m c_sec_terminal = Mode Sec ps)) in
   //let _ = cut (b2t (is_value c_sec_terminal)) in
   //let _ = cut (b2t (Conf.s c_sec_terminal = [])) in
   //let _ = cut (tpre_assec_ret #ps pi_sec_terminal ps) in
 
   //let _ = cut (is_sec c_sec_terminal /\ is_value c_sec_terminal) in
-  let pi_final_par = ret_sec_value_to_ps #ps pi_enter_par c_sec_terminal ps in
+  let pi_final_par = ret_sec_value_to_ps #ps pi_enter_par c_sec ps in
   let pi_final = (pi_final_par, OrdMap.remove ps tsec_terminal) in
 
   (* TODO: FIXME: this also verifies, but with this the whole thing times out *)
   let _ = admitP (eq_proto' ps pi pi_final_par) in
-  ret_sec_value_to_ps_helper_lemma #ps pi_enter_par c_sec_terminal pi_final_par;
+  ret_sec_value_to_ps_helper_lemma #ps pi_enter_par c_sec pi_final_par;
 
-  let s2:pstep #ps pi_sec_terminal pi_final =
-    P_sec_exit #ps pi_sec_terminal ps pi_final in
+  let s2:pstep #ps pi_sec_terminal pi_final = P_sec_exit #ps pi_sec_terminal ps pi_final in
 
-  let h1:pstep_star #ps pi_enter pi_final =
-    pss_ps_to_pss #ps #pi_enter #pi_sec_terminal #pi_final ss s2 in
+  let h1:pstep_star #ps pi_enter pi_final = pss_ps_to_pss #ps #pi_enter #pi_sec_terminal #pi_final ss s2 in
 
-  let h2:pstep_star #ps pi_init pi_final =
-    PS_tran #ps #pi_init #pi_enter #pi_final s1 h1 in
+  let h2:pstep_star #ps pi_init pi_final = PS_tran #ps #pi_init #pi_enter #pi_final s1 h1 in
+  let _ = admitP (pstep_star #ps pi_init pi_final) in
 
-  (| Mk_prop ps x e pi c_sec_terminal pi_init pi_final h2, () |)
+  let _ = cut (pi_init_prop ps (fst pi_init) en_m red_m) in
+  let _ = cut (tpre_assec #ps pi_init ps x e) in
+  let _ = cut (final_prop ps (fst pi_final) c_sec) in
+  let _ = cut (pstep_star #ps pi_init pi_final) in
+  let _ = cut (eq_proto' ps (fst pi_init) (fst pi_final)) in
+  let _ = cut (sec_comp_prop ps en_m red_m x e c_sec (pi_init, pi_final)) in
+
+  let h = get_proof (sec_comp_prop ps en_m red_m x e c_sec (pi_init, pi_final)) in
+
+  (| (pi_init, pi_final), h |)
 
 #reset-options
 
@@ -294,3 +334,16 @@ let handle_connection c_in c_out =
 
 
 (* (\*     //let _ = create_thread (do_sec_comp ps env_m' out_m' x e) in *\) *)
+
+
+(* type sec_prop = *)
+(*   | Mk_prop: *)
+(*     ps:prins -> x:varname -> e:exp *)
+(*     -> pi:tpar ps *)
+(*     -> c_sec_terminal:config{is_sterminal c_sec_terminal} *)
+(*     -> pi_init:protocol ps{pi_init = (pi, (OrdMap.empty #prins #tconfig_sec #ps_cmp)) /\ tpre_assec #ps pi_init ps x e} *)
+(*     -> pi_final:protocol ps *)
+(*     -> h:pstep_star #ps pi_init pi_final{final_prop ps (fst pi_final) c_sec_terminal /\ *)
+(*                                         eq_proto' ps (fst pi_init) (fst pi_final)} *)
+(*     -> sec_prop *)
+
